Reorganize Mceliece and older files.

lib/Crypto/BitVec.lean
@@ -42,9 +42,6 @@ def msbb_fix (m : Nat) (i : Nat) : Nat :=
 
 def msbb_get! (x : BitVec m) (i : Nat) : Bool := x.lsb_get! (msbb_fix m i)
 
-def msbb_set! (x : BitVec m) (i : Nat) (c : Bool) : BitVec m :=
-  x.lsb_set! (msbb_fix m i) c
-
 protected def toBinary (x : BitVec n) : String :=
   let l := Nat.toDigits 2 x.val
   "0b" ++ String.mk (List.replicate (n - l.length) '0' ++ l)
@@ -52,15 +49,6 @@ protected def toBinary (x : BitVec n) : String :=
 protected def toHex (x : BitVec n) : String :=
   let l := Nat.toDigits 16 x.val
   "0x" ++ String.mk (List.replicate (n/4 - l.length) '0' ++ l)
-
-protected def toHex2 (x : BitVec n) : String := Id.run do
-  let mut s : String := "0x"
-  for i in range 0 (n/8) do
-    let b := UInt8.ofNat (x.val >>> (8*i))
-    s := s ++ b.toHex
-  pure s
-
-instance : ToString (BitVec n) := ⟨BitVec.toHex2⟩
 
 def reverse (x : BitVec n) : BitVec n := Id.run do
   let mut r : Nat := 0
@@ -70,10 +58,13 @@ def reverse (x : BitVec n) : BitVec n := Id.run do
       r := r + 1
   pure ⟨r, sorry⟩
 
-protected def foldl (f : α → Bool → α) (x : BitVec n) (a : α) : α := Id.run do
+-- Fold that visits least-significant bit first.
+protected def fold_lsb (f : α → Bool → α) (x : BitVec n) (a : α) : α := Id.run do
   let mut r := a
-  for i in range 0 n do
-    r := f r (x.msbb_get! i)
+  let mut v := x.val
+  for _i in range 0 n do
+    r := f r ((v &&& 1) = 1)
+    v := v >>> 1
   pure r
 
 protected def take_lsb (x : BitVec m) (n : Nat) : BitVec n :=
@@ -82,7 +73,12 @@ protected def take_lsb (x : BitVec m) (n : Nat) : BitVec n :=
 protected def take_msb (x : BitVec m) (n : Nat) : BitVec n :=
   ⟨x.val >>> (m-n), sorry⟩
 
-theorem eq_of_val_eq : ∀ {x y : BitVec n}, x.val = y.val → x = y
+def extractN! (a:BitVec n) (s m:Nat) : BitVec m :=
+  let e := s + m
+  let b := (a.val >>> (n - e)) &&& (1 <<< (min m (n - s)) - 1)
+  ⟨b, sorry⟩
+
+theorem eq_of_val_eq {n:Nat} : ∀{x y : BitVec n}, x.val = y.val → x = y
   | ⟨_,_⟩, _, rfl => rfl
 
 theorem ne_of_val_ne {x y : BitVec n} (h : x.val ≠ y.val) : x ≠ y :=
@@ -111,26 +107,6 @@ protected def generate_msb (n : Nat) (f : Fin n → Bool) : BitVec n := Id.run d
   for i in range 0 n do
     let b := f ⟨i, sorry⟩
     r := r <<< 1 ||| (if b then 1 else 0)
-
-  ⟨r, sorry⟩
-
-protected def generate_msbb (n : Nat) (f : Fin n → Bool) : BitVec n := Id.run do
-  let mut r : Nat := 0
-
-  let m := n % 8
-  if m ≠ 0 then
-    let mut w : Nat := 0
-    for j in range 0 m do
-      let b := f ⟨j, sorry⟩
-      w := if b then 1 <<< j ||| w else w
-    r := w
-
-  for i in range 0 (n/8) do
-    let mut w : Nat := 0
-    for j in range 0 8 do
-      let b := f ⟨m+8*i+j, sorry⟩
-      w := if b then 1 <<< j ||| w else w
-    r := r <<< 8 ||| w
 
   ⟨r, sorry⟩
 
