lib/Crypto/Mceliece/Ref348864.lean
@@ -1,0 +1,802 @@
+import Crypto.Bool
+import Crypto.BitVec
+import Crypto.GF2BV
+import Crypto.GF2Poly
+import Crypto.ByteVec
+import Crypto.Exp
+import Crypto.Matrix
+import Crypto.Nat
+import Crypto.Range
+import Crypto.UInt8
+import Crypto.Vector
+
+def select (c:BitVec n) (t f : Vector n α) : Vector n α :=
+  Vector.generate n (λi => if c.msb_get! i then t.get i else f.get i)
+
+-- `iterN f n a` return `f^n a`.
+def iterN (f : α → α) : Nat → α → α
+| 0, a => a
+| i+1, a => iterN f i (f a)
+
+-- `iterV n f b` returns a pair `(v, r)` where `r`
+def iterV (n:Nat) (f : β → α × β) (b:β) : Vector n α := Id.run do
+  let mut a := Array.mkEmpty n
+  let mut b := b
+  for i in range 0 n do
+    let (v, c) := f b
+    a := a.push v
+    b := c
+  let p : a.size = n := by admit
+  ⟨a, p⟩
+
+def concatByteVec (v : Vector m (ByteVec n)) : ByteVec (m*n) :=
+  let q {i} (p : i < m*n) : i / n < m := sorry
+  let r {i} (p : i < m*n) : 0 < n := sorry
+  ByteVec.generate (m*n) (λi => (v.get ⟨i.val / n, q i.isLt⟩).get (Fin.ofNat' i.val (r i.isLt)))
+
+def concatVec (v : Vector m (Vector n α)) : Vector (m*n) α :=
+  let q {i} (p : i < m*n) : i / n < m := sorry
+  let r {i} (p : i < m*n) : 0 < n := sorry
+  Vector.generate (m*n) (λi => (v.get ⟨i.val / n, q i.isLt⟩).get (Fin.ofNat' i.val (r i.isLt)))
+
+def bitvecToByteVec_msb {r : @&Nat} (w : @&Nat) (v : @&(BitVec r)) : ByteVec w :=
+  ByteVec.generate w λi => Id.run do
+    let mut z : UInt8 := 0
+    for j in range 0 8 do
+      z := z ||| (if v.msb_get! (8*i+j) then (1:UInt8) <<< OfNat.ofNat j else 0)
+    pure z
+
+structure DRBG where
+  key : ByteVec (256 / 8)
+  v : ByteVec (128 / 8)
+
+instance : Inhabited DRBG := ⟨Inhabited.default, Inhabited.default⟩
+
+def tryN {α:Type _ } (f:DRBG → Option α × DRBG) : DRBG → Nat → Option α × DRBG
+  | drbg, 0 =>
+    (none, drbg)
+  | drbg, Nat.succ attempts =>
+    match f drbg with
+    | (some ind, drbg) => (some ind, drbg)
+    | (none, drbg) => tryN f drbg attempts
+
+@[reducible]
+def Seed := ByteVec 48
+
+opaque incrementV (v : ByteVec 16) : ByteVec 16 := Id.run do
+  let mut v := v
+  for i in range 0 15 do
+    let j := 15 - i
+    let vj := v.get! j
+    if vj = 0xff then
+      v := v.set! j 0x00
+    else
+      v := v.add! j 1
+      break
+  pure v
+
+@[extern "lean_AES256_ECB"]
+opaque aes256Ecb (key: @&ByteVec 32) (v: @&ByteVec 16) : ByteVec 16
+
+opaque aes256CtrDrbgUpdate (key : ByteVec 32) (v0 : ByteVec 16) : ByteVec 48 :=
+  let f := λv => let v := incrementV v; (aes256Ecb key v, v)
+  match iterV 3 f v0 with
+  | v => concatByteVec v
+
+opaque randombytesInit (s : Seed) : DRBG :=
+  let key := ByteVec.generate 32 (λ_ => 0)
+  let v   := ByteVec.generate 16 (λ_ => 0)
+  let b := aes256CtrDrbgUpdate key v
+  let b := ByteVec.generate _ (λi => b.get i ^^^ s.get i)
+  { key := b.extractN 0 32, v := b.extractN 32 16 }
+
+private theorem randomBytesTerminates : ∀ n, n ≥ 16 → n - 16 < n := sorry
+
+def randombytes3 (key : ByteVec 32) (v : ByteVec 16) (a : ByteArray) (n : Nat)
+   : ByteArray × ByteVec 16 :=
+  if n == 0 then
+    (a, v)
+  else
+    let v := incrementV v
+    let b := aes256Ecb key v
+    if h : n ≥ 16 then
+      have : n - 16 < n := randomBytesTerminates n ‹_›
+      randombytes3 key v (a ++ b.data) (n - 16)
+    else
+      (a ++ b.data.extractN 0 n, v)
+
+theorem randomBytes3_size (key) (v) (a) (n:Nat)
+    : (randombytes3 key v a n).1.size = n := by
+  admit
+
+opaque randombytes (rbg : DRBG) (n : Nat) : ByteVec n × DRBG :=
+  let key := rbg.key
+  let v := rbg.v
+  let p := randombytes3 key v (ByteArray.mkEmpty n) n
+  let pr : p.1.size = n := randomBytes3_size key v (ByteArray.mkEmpty n) n
+  let b := aes256CtrDrbgUpdate key p.2
+  let rbg := { key := b.extractN 0 32, v := b.extractN 32 16 }
+  (⟨p.1, pr⟩, rbg)
+
+def initKeypairSeedPrefix : ByteVec 1 := #v[64]
+
+def initKeypairSeed (v:ByteVec 32) : ByteVec 33 := initKeypairSeedPrefix ++ v
+
+@[extern "lean_shake256"]
+opaque shake (w:Nat) (input: ByteArray) : ByteVec w
+
+def cryptoHash32b (b:ByteArray) : ByteVec 32 := shake 32 b
+
+namespace Mceliece
+namespace Ref348864
+
+def name : String := "mceliece348864"
+
+def N := 3488
+
+@[reducible]
+def gfbits : Nat := 12
+
+@[reducible]
+def sys_t : Nat := 64
+
+@[reducible]
+def cond_bytes : Nat := (1 <<< (gfbits-4))*(2*gfbits - 1)
+
+@[reducible]
+def pk_nrows : Nat := sys_t * gfbits
+
+@[reducible]
+def pk_ncols : Nat := N - pk_nrows
+
+def publicKeyBytes : Nat := pk_nrows * (pk_ncols / 8)
+
+def PublicKey := Vector pk_nrows (BitVec pk_ncols)
+
+namespace PublicKey
+
+-- Create public key from row matrix
+def init (m : Vector pk_nrows (BitVec N)) : PublicKey :=
+  Vector.generate pk_nrows λr =>
+    (m.get! r).take_lsb pk_ncols
+
+def pk_row_bytes : Nat := pk_ncols / 8
+
+protected
+def toBytes (pk:PublicKey) : ByteVec publicKeyBytes :=
+  let v := bitvecToByteVec_msb (pk_ncols / 8) <$> pk
+  ByteVec.generate publicKeyBytes λi =>
+    let r := i.val / pk_row_bytes
+    let c := i.val % pk_row_bytes
+    (v.get! r).get! c
+
+protected def toString (pk:PublicKey) : String := pk.toBytes.toString
+
+instance : ToString PublicKey := ⟨PublicKey.toString⟩
+
+end PublicKey
+
+@[reducible]
+def GF := { x:UInt16 // x.val < (1<<<12) }
+
+def gfMask : UInt16 := OfNat.ofNat ((1 <<< 12) - 1)
+
+namespace GF
+
+instance (n:Nat) : OfNat GF n where
+  ofNat := ⟨UInt16.ofNat n &&& gfMask, sorry⟩
+
+instance : Inhabited GF := ⟨OfNat.ofNat 0⟩
+
+protected def xor (x y:GF) : GF := ⟨x.val ^^^ y.val, sorry⟩
+
+-- This should compute x * y mod x^12 + x^3 + 1
+protected def red (tmp : UInt32) : GF :=
+  let t := tmp &&& 0x7fc000
+  let tmp := tmp ^^^ (t >>> 9) ^^^ (t >>> 12)
+  let t := tmp &&& 0x3000
+  let tmp := tmp ^^^ (t >>> 9) ^^^ (t >>> 12)
+ ⟨tmp.toUInt16 &&& gfMask, sorry⟩
+
+-- This computes (x * y) mod x^12 + x^3 + 1
+protected def mul (x y : GF) : GF := Id.run do
+  let x : UInt32 := x.val.toUInt32
+  let y : UInt32 := y.val.toUInt32
+  let mut tmp : UInt32 := 0
+  for i in [0:12] do
+    let mask : UInt32 := 1 <<< (UInt32.ofNat i)
+    opaque tmp := tmp ^^^ (x * (y &&& mask))
+  return GF.red tmp
+
+instance : Xor GF := ⟨GF.xor⟩
+instance : Add GF := ⟨GF.xor⟩
+instance : Sub GF := ⟨GF.xor⟩
+instance : Mul GF := ⟨GF.mul⟩
+
+-- This computes (x * x) mod x^12 + x^3 + 1
+def sq (x:GF) : GF :=
+  let x := x.val.toUInt32
+  let x := (x ||| (x <<< 8)) &&& 0x00FF00FF
+  let x := (x ||| (x <<< 4)) &&& 0x0F0F0F0F
+  let x := (x ||| (x <<< 2)) &&& 0x33333333
+  let x := (x ||| (x <<< 1)) &&& 0x55555555
+  GF.red x
+
+-- This computes x^-1 (mod x^12 + x^3 + 1)
+def inv (i:GF) : GF :=
+  let tmp11 := i.sq * i                  -- 11
+  let tmp1111 := tmp11.sq.sq * tmp11     -- 1111
+  let o := tmp1111.sq.sq.sq.sq * tmp1111 -- 11111111
+  let o := o.sq.sq * tmp11               -- 1111111111
+  let o := o.sq * i                      -- 11111111111
+  o.sq                                   -- 111111111110
+
+protected def div (n d : GF) := n * d.inv
+
+instance : Div GF := ⟨GF.div⟩
+
+instance : CommMulMonoid GF where
+  mul_assoc := sorry
+  mul_comm  := sorry
+  mul_one := sorry
+
+protected def bit (x:GF) (idx:Nat) : Bool :=
+  if idx < 12 then
+    (x.val >>> UInt16.ofNat idx) &&& 1 = 1
+  else
+    false
+
+def bitrev (x:GF) : GF :=
+  let a : UInt16 := x.val
+  let a := ((a &&& 0x00FF) <<< 8) ||| ((a &&& 0xFF00) >>> 8)
+  let a := ((a &&& 0x0F0F) <<< 4) ||| ((a &&& 0xF0F0) >>> 4)
+  let a := ((a &&& 0x3333) <<< 2) ||| ((a &&& 0xCCCC) >>> 2)
+  let a := ((a &&& 0x5555) <<< 1) ||| ((a &&& 0xAAAA) >>> 1)
+  ⟨a >>> 4, sorry⟩
+
+end GF
+
+def loadGf {n} (r: ByteVec n) (i:Nat) : GF :=
+  let f (x:UInt8) : UInt16 := UInt16.ofNat x.toNat
+  let w : UInt16 := f (r.get! (i+1)) <<< 8 ||| f (r.get! i)
+  ⟨w &&& gfMask, sorry⟩
+
+def loadGfArray {n:Nat} (r: ByteVec (2*n)) : Vector n GF :=
+  Vector.generate n (λi => loadGf r (2*i.val))
+
+@[extern "lean_store_gf"]
+opaque store_gf (irr : Vector sys_t GF) : ByteVec (2*sys_t)
+
+def secretKeyBytes : Nat := 40 + 2*sys_t + cond_bytes + N/8
+
+@[extern "lean_controlbitsfrompermutation2"]
+opaque controlBitsFromPermutation2 (pi : @&Vector (1 <<< gfbits) GF) : ByteVec cond_bytes
+
+theorem shl_plus_shl (n : Nat) : (1 <<< n + 1 <<< n) = 1 <<< (n+1) := sorry
+
+theorem shl_times_shl (m n : Nat) : (1 <<< m * 1 <<< n) = 1 <<< (m+n) := sorry
+
+def layer (pi : Vector (1 <<< gfbits) GF) (cb : BitVec (1 <<< gfbits)) (s : Fin gfbits) : Vector (1 <<< gfbits) GF :=
+  let si := s.val
+  let stride := 1 <<< si
+  let h : Vector (1 <<< (gfbits - (si+1)) * (1 <<< si + 1 <<< si)) GF = Vector (1 <<< gfbits) GF := by
+        apply congrFun
+        apply congrArg
+        simp only [shl_plus_shl, shl_times_shl, Nat.sub_add_cancel s.isLt]
+  cast h $
+    concatVec $ Vector.generate (1 <<< (gfbits - (s+1))) λk =>
+      let i := stride*k.val
+      let c  : BitVec (1 <<< si) := cb.extractN! i stride
+      let p1 : Vector (1 <<< si) GF := pi.extractN! (2*i) stride
+      let p2 : Vector (1 <<< si) GF := pi.extractN! (2*i+stride) stride
+      select c p2 p1 ++ select c p1 p2
+
+def testPerm (out : ByteVec cond_bytes) :  Vector (1 <<< gfbits) GF := Id.run do
+  let w  := gfbits
+  let n  := 1 <<< gfbits
+  let n4 := n >>> 4
+  let out :=
+        Vector.generate (2*w-1) λi =>
+          let cb := out.extractN (n4 * i) n4
+          BitVec.generate_msb (1 <<< gfbits) λi => (cb.get! (i.val/8)).testBit (i.val%8)
+  let mut pi := Vector.generate n (λi => (OfNat.ofNat i.val : GF))
+  for i in range 0 w do
+    let cb := out.get! i
+    pi := layer pi cb ⟨i, sorry⟩
+  for j in range 0 (w-1) do
+    let cb := out.get! (w+j)
+    let i := (w - 2) - j
+    pi := layer pi cb ⟨i, sorry⟩
+  pure pi
+
+def controlBitsFromPermutation (pi : Vector (1 <<< gfbits) GF) : Option (ByteVec cond_bytes) :=
+  let out := controlBitsFromPermutation2 pi
+  if pi ≠ testPerm out then
+    none
+  else
+    some out
+
+structure SecretKey where
+  seed : ByteVec 32
+  goppa : Vector sys_t GF
+  permutation : Vector (1 <<< gfbits) GF
+  controlbits : ByteVec cond_bytes
+  rest : ByteVec (N/8)
+
+namespace SecretKey
+
+def byteVec (sk:SecretKey) : ByteVec secretKeyBytes :=
+  sk.seed
+    ++ ByteVec.ofUInt64lsb 0xffffffff
+    ++ store_gf sk.goppa
+    ++ sk.controlbits
+    ++ sk.rest
+
+protected def toString (sk:SecretKey) : String := sk.byteVec.toString
+
+instance : ToString SecretKey := ⟨SecretKey.toString⟩
+
+end SecretKey
+
+structure KeyPair where
+  pk : PublicKey
+  sk : SecretKey
+
+@[reducible]
+def rw : Nat :=  N/8 + 4*(1 <<< gfbits) + sys_t * 2 + 32
+
+def byteToUInt32 (v:UInt8) : UInt32 := UInt32.ofNat (v.toNat)
+
+def load4 {n} (r: ByteVec n) (i:Nat) : UInt32 :=
+  let b (j:Nat) (s:UInt32) : UInt32 := byteToUInt32 (r.get! (i+j)) <<< s
+  b 0 0 ||| b 1 8 ||| b 2 16 ||| b 3 24
+
+def load4Array {n:Nat} (r: ByteVec (4*n)) : Vector n UInt32 :=
+  Vector.generate n (λi => load4 r (4*i.val))
+
+def poly_full_mul {m n:Nat} {α:Type _} [Add α] [Mul α] [OfNat α 0] (x : Vector m α) (y : Vector n α) : Vector (m+n-1) α := Id.run do
+  let mut prod : Vector (m+n-1) α := Vector.replicate (m+n-1) 0
+  let _h : Inhabited α := ⟨0⟩
+  for i in range 0 m do
+    for j in range 0 n do
+      prod := prod.set! (i+j) (prod.get! (i+j) + x.get! i * y.get! j)
+  pure prod
+
+def GF_red (z : Vector (2*sys_t-1) GF) : Vector sys_t GF := Id.run do
+  let mut z := z
+  for j in range 0 (sys_t-1) do
+    let i := sys_t-2 - j
+    let p := z.get! (sys_t+i)
+    z := z.sub! (i+3) p
+    z := z.sub! (i+1) p
+    z := z.sub! (i+0) (2*p)
+  pure (Vector.generate sys_t λi => z.get! i)
+
+def GF_mul (x y : Vector sys_t GF) : Vector sys_t GF :=
+  GF_red (@poly_full_mul sys_t sys_t GF _ _ _ x y)
+
+def genPolyGen_mask (mat : Matrix (sys_t+1) sys_t GF) (j:Nat) : GF := Id.run do
+  let mut r := mat.get! j j
+  for i in rangeH j (sys_t+1) do
+    for k in rangeH (j+1) sys_t do
+      r := r ^^^ mat.get! i k
+  pure r
+
+def genPolyGenUpdate (mat : Matrix (sys_t+1) sys_t GF) (j : Nat) (inv : GF)
+    : Matrix (sys_t+1) sys_t GF :=
+  Matrix.generate _ _ λr c =>
+    if r ≤ j then
+      0
+    else
+      if c = j then
+        inv * mat.get! r j
+      else
+        mat.get! r c ^^^ (inv * mat.get! r j * mat.get! j c)
+
+def genPolyGen (f : Vector sys_t GF) : Option (Vector sys_t GF) := Id.run do
+  let v0 : Vector sys_t GF := Vector.generate sys_t λi => if i = 0 then 1 else 0
+  let mut mat := Matrix.unfoldBy (GF_mul f) v0
+  for j in range 0 sys_t do
+    let mut r := mat.get! j j
+    if r = 0 then
+      r := genPolyGen_mask mat j
+    if r = 0 then
+      return none
+    else
+      mat := genPolyGenUpdate mat j r.inv
+  some (mat.row! sys_t)
+
+-- Map used by init_pi
+structure Perm where
+  value : UInt32
+  idx : GF
+
+namespace Perm
+
+instance : Inhabited Perm := ⟨{ value := 0, idx := 0}⟩
+
+end Perm
+
+-- Generate random permutation from random uint32 array
+def randomPermutation (perm : Vector (1 <<< gfbits) UInt32)
+  : Option (Vector (1 <<< gfbits) GF) := Id.run do
+  -- Build vector associated input number to index
+  let v : Vector (1 <<< gfbits) Perm :=
+        Vector.generate _
+          (λi => { value := perm.get i, idx := OfNat.ofNat i.val })
+
+  -- Sort vector based on value to get random permutation
+  let lt (x y : Perm) : Bool := x.value < y.value
+  let v : Vector (1 <<< gfbits) Perm := Vector.qsort v lt
+
+  -- Check to see if we have duplicated values in sorted array
+  -- Failing to check can bias result
+  for i in range 0 (1 <<< gfbits - 1) do
+    if (v.get! i).value = (v.get! (i+1)).value then
+      return none
+
+  pure (some (Perm.idx <$> v))
+
+def eval (f : Vector (sys_t+1) GF) (a : GF) : GF := Id.run do
+  let mut r := f.get! sys_t
+  for j in range 0 sys_t do
+    r := r * a
+    r := r + f.get! (sys_t - 1 - j)
+  pure r
+
+def init_mat_row (inv : Vector N GF) (k : Nat) : BitVec N :=
+  BitVec.generate_msb N λi =>
+    let gf := inv.get i
+    gf.bit k
+
+def flatten [Inhabited α] (v : Vector m (Vector n α)) : Vector (m*n) α :=
+  Vector.generate (m*n) λi => (v.get! (i.val/n)).get! (i.val%n)
+
+def init_mat (g : Vector sys_t GF) (L : Vector N GF) : Vector pk_nrows (BitVec N) := Id.run do
+  let g' := g.push 1
+  let inv0 := (λx => (eval g' x).inv) <$> L
+  flatten $
+    Vector.generate sys_t λi =>
+      let inv := Vector.generate N λj =>
+            inv0.get! j * exp (L.get! j) i
+      Vector.generate gfbits λk => init_mat_row inv k
+
+def gaussian_elim_row (m : Vector pk_nrows (BitVec N)) (row: Nat)
+  : Option (Vector pk_nrows (BitVec N)) := Id.run do
+  let mut mat_row : BitVec N := m.get! row
+  for k in rangeH (row+1) pk_nrows do
+    let mat_k := m.get! k
+    let mask1 := mat_row.msb_get! row
+    let mask2 := mat_k.msb_get! row
+    if mask1 ≠ mask2 then
+      mat_row := mat_row ^^^ mat_k
+  if not (mat_row.msb_get! row) then
+    return none
+  let mut m := m
+  for k in range 0 pk_nrows do
+    if k = row then
+      m := m.set! k mat_row
+    else
+      let mat_k := m.get! k
+      if mat_k.msb_get! row then
+        m := m.set! k (mat_k ^^^ mat_row)
+  pure (some m)
+
+def gaussian_elim (m : Vector pk_nrows (BitVec N))
+  : Option (Vector pk_nrows (BitVec N)) := Id.run do
+  let mut m := m
+  for i in range 0 pk_nrows do
+    match gaussian_elim_row m i with
+    | some m1 =>
+      m := m1
+    | none => return none
+  pure (some m)
+
+def mkPublicKey (g : Vector sys_t GF) (pi: Vector (1 <<< gfbits) GF) : Option PublicKey := do
+  let L   := Vector.generate N λi => (pi.get! i).bitrev
+  PublicKey.init <$> gaussian_elim (init_mat g L)
+
+def tryCryptoKemKeypair (seed: ByteVec 32) (r: ByteVec rw) : Option KeyPair := do
+  let g ← genPolyGen $ loadGfArray $ r.extractN (N/8 + 4*(1 <<< gfbits)) (2*sys_t)
+  let pi ← randomPermutation $ load4Array $ r.extractN (N/8) (4*(1 <<< gfbits))
+  let cb ← controlBitsFromPermutation pi
+  let pk ← mkPublicKey g pi
+  let sk := { seed := seed,
+              goppa := g,
+              permutation := pi,
+              controlbits := cb,
+              rest := r.extractN 0 (N/8)
+            }
+  some { pk := pk, sk := sk }
+
+def mkCryptoKemKeypair (iseed : Seed) (attempts: optParam Nat 10) : Option (KeyPair × DRBG) := do
+  let rec loop : ByteVec 32 → Nat → Option KeyPair
+      | _, 0 => none
+      | seed, Nat.succ n => do
+        let r := shake rw (#v[64] ++ seed).data
+        match tryCryptoKemKeypair seed r with
+        | some kp => some kp
+        | none =>
+          loop (r.takeFromEnd 32) n
+  let drbg := randombytesInit iseed
+  let (bytes, drbg) := randombytes drbg 32
+  match loop bytes attempts with
+  | none => none
+  | some p => some (p, drbg)
+
+def tryGenerateRandomErrors (v : Vector (2*sys_t) GF) (n:Nat) : Option (Vector n (Fin N)) := Id.run do
+  let mut ind : Array (Fin N) := Array.mkEmpty sys_t
+  for num in v.data do
+    let num := num.val.toNat
+    if lt : num < N then
+      ind := ind.push ⟨num, lt⟩
+      if eq:ind.size = n then
+        return (some ⟨ind, eq⟩)
+  pure none
+
+def has_duplicate {n:Nat} {α:Type} [DecidableEq α] (v: Vector n α) : Bool := Id.run do
+  for i in rangeH 1 n do
+    for j in range 0 i do
+      if lt_i : i < n then
+        if lt_j : j < n then
+          if v.get ⟨i, lt_i⟩ = v.get ⟨j, lt_j⟩ then
+            return true
+  pure false
+
+def generateErrorBitmask (a: Vector sys_t (Fin N)) : BitVec N := Id.run do
+  let mut e : BitVec N := BitVec.zero N
+  for v in a.data do
+    e := e.msb_set! v.val true
+  pure e
+
+def tryGenerateErrors (drbg:DRBG) : Option (BitVec N) × DRBG := Id.run do
+  let (bytes, drbg) := randombytes drbg (4*sys_t)
+  let input : Vector (2*sys_t) GF := loadGfArray bytes
+
+  let mut a : Array (Fin N) := Array.mkEmpty sys_t
+  for (num : GF) in input.data do
+    let num : Nat := num.val.toNat
+    if lt : num < N then
+      a := a.push ⟨num, lt⟩
+      -- Check to see if done
+      if eq:a.size = sys_t then
+        let v : Vector sys_t (Fin N) := ⟨a, eq⟩
+        if has_duplicate v then
+          return (none, drbg)
+        return (some (generateErrorBitmask v), drbg)
+  pure ⟨none, drbg⟩
+
+def cSyndrome (pk : PublicKey) (e: BitVec N) : BitVec pk_nrows := Id.run do
+  BitVec.generate_msb pk_nrows λi =>
+    let off := (BitVec.zero pk_nrows).msb_set! i True
+    let row : BitVec N := off ++ pk.get! i
+    (row &&& e).fold_lsb (· ^^^ ·) false
+
+@[reducible]
+structure Ciphertext where
+  syndrome : BitVec pk_nrows
+  hash : ByteVec 32
+
+namespace Ciphertext
+
+protected def bytes (c:Ciphertext) : ByteVec 128 :=
+  bitvecToByteVec_msb (pk_nrows/8) c.syndrome ++ c.hash
+
+protected def toString (c:Ciphertext) : String := c.bytes.toString
+
+instance : ToString Ciphertext := ⟨Ciphertext.toString⟩
+
+def mkHash (e:BitVec N) : ByteVec 32 :=
+  cryptoHash32b (ByteArray.fromList [2] ++ (bitvecToByteVec_msb (N/8) e).data)
+
+end Ciphertext
+
+structure Plaintext where
+  e : BitVec N
+  c : Ciphertext
+
+namespace Plaintext
+
+protected def bytes (p:Plaintext) :  ByteVec 32 :=
+  cryptoHash32b (ByteArray.fromList [1] ++ (bitvecToByteVec_msb (N/8) p.e).data ++ p.c.bytes.data)
+
+protected def toString (p:Plaintext) : String := p.bytes.toString
+
+instance : ToString Plaintext := ⟨Plaintext.toString⟩
+
+end Plaintext
+
+structure EncryptionResult where
+  e : BitVec N
+  ct : Ciphertext
+
+def EncryptionResult.ss (r:EncryptionResult) : Plaintext := { e := r.e, c := r.ct }
+
+def mkCryptoKemEnc (drbg:DRBG) (attempts:Nat) (pk:PublicKey) : Option (EncryptionResult × DRBG) := do
+  match tryN tryGenerateErrors drbg attempts with
+  | (some e, drbg) =>
+    let c   := { syndrome := cSyndrome pk e,
+                 hash := Ciphertext.mkHash e
+                }
+    some ({ e := e, ct := c }, drbg)
+  | (none, _) => panic! "mkCryptoKemEnc def failure"
+
+@[extern "lean_transpose64"]
+opaque tranpose64 (a : @&(Vector 64 UInt64)) : Vector 64 UInt64
+
+def load4_64
+  (c : ByteVec 256)
+  : Vector 64 UInt64 :=
+  Vector.generate 64 $ λi => Id.run do
+    let mut r := 0
+    for j in range 0 4 do
+      r := (r <<< 8) ||| (c.get! (4*i+3-j)).toNat
+    pure $ UInt64.ofNat r
+
+def benes_layer
+  (data : @&(Vector 64 UInt64))
+  (bits : @&(Vector 32 UInt64))
+  (lgs : @&Nat)
+    : Vector 64 UInt64 := Id.run do
+  let s : Nat := 1 <<< lgs
+  let mut data := data
+  for h2 in range 0 (32 >>> lgs) do
+    let h := h2 <<< lgs
+    for k in range 0 s do
+      let j := 2 * h + k
+      let d := (data.get! j ^^^ data.get! (j+s)) &&& bits.get! (h+k)
+      data := data.xor! j d
+      data := data.xor! (j+s) d
+  pure data
+
+def slice {m:Nat} (v:ByteVec m) (l n : Nat) : ByteVec n :=
+  ByteVec.generate n (λi => v.get! (l+i))
+
+def load8 (n:Nat) : UInt64 := Id.run do
+  let mut r := 0
+  for j in range 0 8 do
+    r := (r <<< 8) ||| ((n >>> (8*j)) &&& 0xff)
+  pure $ UInt64.ofNat r
+
+def load8_32 (c: ByteVec 256) : Vector 32 UInt64 :=
+  Vector.generate 32 $ λi => Id.run do
+    let mut r := 0
+    for j in range 0 8 do
+      r := (r <<< 8) ||| (c.get! (8*i+(7-j))).toNat
+    pure $ UInt64.ofNat r
+
+def apply_benes0 (a0 : Vector 64 UInt64)
+                 (c : ByteVec cond_bytes)
+    : Vector 64 UInt64 := Id.run do
+  let inc := 256
+
+  let mut a := a0
+  a := tranpose64 a
+  for l in range 0 6 do
+    let c := slice c (inc*l) inc
+    let c := load4_64 c
+    let c := tranpose64 c
+    let c := Vector.generate 32 (λi => c.get! i)
+    a := benes_layer a c l
+  a := tranpose64 a
+  for i in range 0 6 do
+    let c := slice c (inc*(6+i)) inc
+    a := benes_layer a (load8_32 c) i
+  for j in range 0 5 do
+    let i := 4 - j
+    let c := slice c (inc*(16-i)) inc
+    a := benes_layer a (load8_32 c) i
+  a := tranpose64 a
+  for j in range 0 6 do
+    let l := 5 - j
+    let c := slice c (inc*(22-l)) inc
+    let c := load4_64 c
+    let c := tranpose64 c
+    let c := Vector.generate 32 (λi => c.get! i)
+    a := benes_layer a c l
+  pure <| tranpose64 a
+
+def support_gen (c : ByteVec cond_bytes) : Vector N GF := Id.run do
+  let L : Vector gfbits (Vector 64 UInt64) :=
+        Vector.generate gfbits λj =>
+          let r :=
+            BitVec.generate_lsb (1 <<< gfbits) λ(i : Fin (1 <<< gfbits)) =>
+              let i : GF := OfNat.ofNat i.val
+              i.bit (11-j)
+          let a0 :=
+            Vector.generate 64 (λi =>
+              UInt64.ofNat ((r.val >>> (64*i.val)) &&& (2^64 - 1)))
+          apply_benes0 a0 c
+  Vector.generate N λi0 => Id.run do
+    let i  := i0.val / 64
+    let m2 := i0.val % 64
+    let mut si : Nat := 0
+    for k in range 0 gfbits do
+      let r := L.get! (gfbits-1-k)
+      let e := ((r.get! i).toNat >>> m2) &&& 1
+      si := si <<< 1 ||| e
+    pure (OfNat.ofNat si)
+
+def synd
+    (g: Vector sys_t GF)
+    (l : Vector N GF)
+    (error_bitmask : BitVec N)
+   : Vector (2*sys_t) GF := Id.run do
+  let mut out := Vector.replicate (2*sys_t) 0
+  let f := g.push 1
+  for i in range 0 N do
+    if error_bitmask.msb_get! i then
+      let e := eval f (l.get! i)
+      let mut e_inv := (e * e).inv
+      for j in range 0 (2*sys_t) do
+        out := out.set! j (out.get! j + e_inv)
+        e_inv := e_inv * l.get! i
+  pure out
+
+-- the Berlekamp-Massey algorithm
+-- input: s, sequence of field elements
+-- output: out, minimal polynomial of s
+def bm
+    (s: Vector (2*sys_t) GF)
+   : Vector (sys_t+1) GF := Id.run do
+  let mut B := Vector.generate (sys_t+1) λi => if i = 1 then 1 else 0
+  let mut C := Vector.generate (sys_t+1) λi => if i = 0 then 1 else 0
+  let mut L : Nat := 0
+  let mut b : GF := 1
+  for N in range 0 (2*sys_t) do
+    let mut d : GF := 0
+    for i in range 0 (min N sys_t + 1) do
+      d := d + (C.get! i * s.get! (N-i))
+
+    if d ≠ 0 then
+      let T := C
+      C := C + (d/b) * B
+      if N ≥ 2*L then
+        L := N+1-L
+        B := T
+        b := d
+    B := Vector.generate (sys_t+1) λi =>
+           if i = 0 then 0 else B.get! (i-1)
+  pure $ Vector.generate (sys_t+1) λi => C.get ⟨sys_t-i, sorry⟩
+
+-- Decrypt the N-bit vector created by mkCryptoKemEnc
+def cryptoKemDec1 (c : Ciphertext) (sk : SecretKey) : Option (BitVec N) := do
+  let g := sk.goppa
+  let l : Vector N GF := support_gen sk.controlbits
+  let r : BitVec N := c.syndrome ++ BitVec.zero (N-pk_nrows)
+  let s := synd g l r
+  let locator := bm s
+  let images := (λi => (eval locator i).inv) <$> l
+
+  let mut w : Nat := 0
+  for i in range 0 N do
+    if images.get! i = 0 then
+      w := w + 1
+  let e : BitVec N := BitVec.generate_msb N λi => images.get i = 0
+  -- Generate preimage
+  if w = sys_t ∧ Ciphertext.mkHash e = c.hash ∧ s = synd g l e then
+    some e
+  else
+    none
+
+-- This is the basic correctness theorem that if we
+-- make a public key from Goppa polynomial and permutation
+-- and use that to generate an encryption key result, then
+-- we can decrypt it.
+theorem decryptEncrypt (drbg drbg' : DRBG)
+               (attempts : Nat)
+               (sk: SecretKey)
+               (pk : PublicKey)
+               (r:EncryptionResult) :
+    controlBitsFromPermutation sk.permutation = some sk.controlbits
+    → mkPublicKey sk.goppa sk.permutation = some pk
+    → mkCryptoKemEnc drbg attempts pk = some (r, drbg')
+    → cryptoKemDec1 r.ct sk = some r.e := by
+  admit
+
+def cryptoKemDec (c : Ciphertext) (sk : SecretKey) : Option Plaintext := do
+  let e ← cryptoKemDec1 c sk
+  some $ { e := e, c := c }
+
+end Ref348864
+end Mceliece
